Updates

generic/Zeta.AppSimulate.Helper.fsti
@@ -119,3 +119,42 @@ val lemma_valid_empty (#app:_) (fs: seq (appfn_call app){length fs = 0})
 
 val lemma_init_value_null (#app:_) (fs: seq (appfn_call app){length fs = 0}) (k: app_key app.adm)
   : Lemma (ensures (post_state fs k = Null))
+
+val empty_call_result_valid (#app:_) (rs: seq (appfn_call_res app))
+  : Lemma (ensures (length rs = 0 ==> valid_call_result rs))
+
+let app_fcs_empty (#app:_) (fcrs: seq (appfn_call_res app))
+  : Lemma (ensures (length fcrs = 0 ==> length (app_fcs fcrs) = 0))
+   = ()
+
+let app_fcs_snoc (#app:_) (fcrs: seq (appfn_call_res app) {length fcrs > 0})
+  : Lemma (ensures (let i = length fcrs - 1 in
+                    let fcrs' = prefix fcrs i in
+                    let fc = to_app_fc fcrs i in
+                    app_fcs fcrs = append1 (app_fcs fcrs') fc))
+  = let i = length fcrs - 1 in
+    let fcrs' = prefix fcrs i in
+    let fcs = app_fcs fcrs in
+    let fcs' = app_fcs fcrs' in
+    let fc = to_app_fc fcrs i in
+    let fcs2 = append1 fcs' fc in
+    let aux (i:_)
+      : Lemma (ensures (index fcs i = index fcs2 i))
+      = ()
+    in
+    FStar.Classical.forall_intro aux;
+    assert(equal fcs fcs2)
+
+val valid_call_result_snoc (#app:_) (fcrs: seq (appfn_call_res app) {length fcrs > 0})
+  : Lemma (requires (let i = length fcrs - 1  in
+                     let fcrs' = prefix fcrs i in
+                     valid_call_result fcrs'))
+          (ensures (let i = length fcrs - 1 in
+                    let fcrs' = prefix fcrs i in
+                    let fcs' = app_fcs fcrs' in
+                    let st' = post_state fcs' in
+                    let fc = to_app_fc fcrs i in
+                    let fcr = index fcrs i in
+                    succeeds fc st' ==>
+                    fcr.res_cr = result fc ==>
+                    valid_call_result fcrs))
